The simple example works again

src/examples/simple.v
@@ -8,7 +8,7 @@ From self.lang Require Import notation lang.
 From self.algebra Require Import view.
 From self.base Require Import primitive_laws class_instances.
 From self.high Require Import proofmode wpc_proofmode.
-From self.high Require Import dprop resources crash_weakestpre weakestpre recovery_weakestpre lifted_modalities.
+From self.high Require Import dprop resources crash_weakestpre weakestpre recovery_weakestpre lifted_modalities post_crash_modality.
 
 Instance subseteq_nat : SqSubsetEq nat := λ v w, v ≤ w.
 
@@ -70,7 +70,7 @@ End specs.
 Section simple_increment.
   Context `{!nvmFixedG Σ, nvmDeltaG Σ}.
 
-  Definition incr (ℓa ℓb : loc) : expr :=
+  Definition incr_both (ℓa ℓb : loc) : expr :=
     #ℓa <- #1 ;;
     WB #ℓa ;;
     Fence ;;
@@ -86,89 +86,129 @@ Section simple_increment.
   (* NOTE: This example is currently broken since the crash condition used is
   not objective. We should use the post crash modality in the crash condition
   (maybe built in to WPC). *)
-  (*
   Lemma wp_incr ℓa ℓb n E (Φ : val → dProp Σ) :
-    ⊢ ℓa ↦ []; [0] | (λ s v, ⌜v = #s⌝) -∗
-      ℓb ↦ []; [0] | (λ s v, ⌜v = #s⌝ ∗ know_flush_lb ℓa s) -∗
-      WPC (incr ℓa ℓb) @ n; E
-        {{ λ _,
-           ℓa ↦ []; [0; 1] | (λ s v, ⌜v = #s⌝) ∗ (* FIXME: The [0] should be moved left. *)
-           ℓb ↦ []; [0; 1] | (λ s v, ⌜v = #s⌝ ∗ know_flush_lb ℓa s)
-        }}
-        {{ ∃ (sa1 sa2 sb1 sb2 : list nat),
-           ℓa ↦ sa1; sa2 | (λ s v, ⌜v = #s⌝) ∗
-           ℓb ↦ sb1; sb2 | (λ s v, ⌜v = #s⌝ ∗ know_flush_lb ℓa s) }}.
+    ⊢ ⎡ know_pred ℓa (λ (n : nat) v, ⌜v = #n⌝) ⎤ -∗
+      ⎡ know_pred ℓb (λ (n : nat) v, ⌜v = #n⌝ ∗ know_flush_lb ℓa n) ⎤ -∗
+      ℓa ↦ₚ [0] -∗
+      ℓb ↦ₚ [0] -∗
+      WPC (incr_both ℓa ℓb) @ n; E
+        {{ λ _, ℓa ↦ₚ [0; 1] ∗ ℓb ↦ₚ [0; 1] }}
+        {{ <PC> _, ∃ (sa sb : list nat), ℓa ↦ₚ sa ∗ ℓb ↦ₚ sb }}.
   Proof.
-    iIntros "aPts bPts".
-    rewrite /incr.
+    iIntros "#pred1 #pred2 aPts bPts".
+    rewrite /incr_both.
 
     (* The first store *)
     wpc_bind (_ <- _)%E.
     iApply wpc_atomic_no_mask.
-    iSplit. { iModIntro. iExists _, _, _, _. iFrame "aPts bPts". }
+    iSplit. {
+      iModIntro. iCrash.
+      (* iDestruct "pred1" as "-#pred1". iDestruct "pred2" as "-#pred2". *)
+      iDestruct "aPts" as (? ?) "aPts".
+      iDestruct "bPts" as (? ?) "bPts".
+      iExists _, _. iFrame. }
     iApply (wp_store_ex with "[$aPts]").
     { reflexivity. }
-    { suff H : (0 ≤ 1); first apply H. lia. }
-    { done. }
+    { suff leq : (0 ≤ 1); first apply leq. lia. }
+    { iFrame "pred1". done. }
     simpl.
     iNext. iIntros "aPts".
-    iSplit. { iModIntro. iModIntro. iExists _, _, _, _. iFrame. }
+    iSplit. {
+      iModIntro. iModIntro. iCrash.
+      iDestruct "aPts" as (? ?) "aPts".
+      iDestruct "bPts" as (? ?) "bPts".
+      iExists _, _. iFrame. }
     iModIntro.
     wpc_pures.
-    { iModIntro. iExists _, _, _, _. iFrame. }
+    { iModIntro. iCrash.
+      iDestruct "aPts" as (? ?) "aPts".
+      iDestruct "bPts" as (? ?) "bPts".
+      iExists _, _. iFrame. }
 
     (* The write back *)
     wpc_bind (WB _)%E.
     iApply wpc_atomic_no_mask.
-    iSplit. { iModIntro. iExists _, _, _, _. iFrame "aPts bPts". }
+    iSplit. {
+      iModIntro. iCrash.
+      iDestruct "aPts" as (? ?) "aPts".
+      iDestruct "bPts" as (? ?) "bPts".
+      iExists _, _. iFrame. }
     iApply (wp_wb_ex with "aPts"); first reflexivity.
     iNext.
     iIntros "[aPts afterFence]".
-    iSplit. { iModIntro. iModIntro. iExists _, _, _, _. iFrame "aPts bPts". }
+    iSplit. {
+      iClear "afterFence". (* FIXME: [iModIntro] spins in the absence of this. *)
+      iModIntro. iModIntro. iCrash.
+      iDestruct "aPts" as (? ?) "aPts".
+      iDestruct "bPts" as (? ?) "bPts".
+      iExists _, _. iFrame. }
     iModIntro.
     wpc_pures.
-    { iModIntro. iExists _, _, _, _. iFrame. }
+    { iClear "afterFence". (* FIXME: [iModIntro] spins in the absence of this. *)
+      iModIntro. iCrash.
+      iDestruct "aPts" as (? ?) "aPts".
+      iDestruct "bPts" as (? ?) "bPts".
+      iExists _, _. iFrame. }
 
     (* The fence. *)
     wpc_bind (Fence)%E.
     iApply wpc_atomic_no_mask.
-    iSplit. { iModIntro. iExists _, _, _, _. iFrame "aPts bPts". }
+    iSplit. {
+      iClear "afterFence". (* FIXME: [iModIntro] spins in the absence of this. *)
+      iModIntro. iCrash.
+      iDestruct "aPts" as (? ?) "aPts".
+      iDestruct "bPts" as (? ?) "bPts".
+      iExists _, _. iFrame. }
     iApply (wp_fence with "afterFence").
     iNext.
     iIntros "#pLowerBound".
-    iSplit. { iModIntro. iModIntro. iExists _, _, _, _. iFrame "aPts bPts". }
+    iSplit. {
+      iModIntro. iModIntro. iCrash.
+      iDestruct "aPts" as (? ?) "aPts".
+      iDestruct "bPts" as (? ?) "bPts".
+      iExists _, _. iFrame. }
     iModIntro.
     wpc_pures.
-    { iModIntro. iExists _, _, _, _. iFrame. }
+    { iModIntro. iCrash.
+      iDestruct "aPts" as (? ?) "aPts".
+      iDestruct "bPts" as (? ?) "bPts".
+      iExists _, _. iFrame. }
 
     (* The last store *)
     iApply wpc_atomic_no_mask.
-    iSplit. { iModIntro. iExists _, _, _, _. iFrame "aPts bPts". }
+    iSplit.
+    { iModIntro. iCrash.
+      iDestruct "aPts" as (? ?) "aPts".
+      iDestruct "bPts" as (? ?) "bPts".
+      iExists _, _. iFrame. }
     iApply (wp_store_ex with "[$bPts]").
     { reflexivity. }
-    { suff H : (0 ≤ 1); first apply H. lia. }
-    { iFrame "#". done. }
+    { suff leq : (0 ≤ 1); first apply leq. lia. }
+    { iFrame "#". iFrame "pLowerBound". done. }
     iNext. iIntros "bPts".
-    iSplit. { iModIntro. iModIntro. iExists _, _, _, _. iFrame "aPts bPts". }
+    iSplit. {
+      iModIntro. iModIntro. iCrash.
+      iDestruct "aPts" as (? ?) "aPts".
+      iDestruct "bPts" as (? ?) "bPts".
+      iExists _, _. iFrame. }
     iModIntro.
     iFrame "aPts bPts".
   Qed.
-  *)
 
   (* FIXME: Hoare triples don't work as Perennial's Hoare triples are tied to iProp. *)
   (* Lemma wpc_incr' (ℓa ℓb : loc) : *)
   (*   {{{ (True : dProp Σ) }}} *)
-  (*     incr ℓa ℓb @ 10; ⊤ *)
+  (*     incr_both ℓa ℓb @ 10; ⊤ *)
   (*   {{{ RET #(); (True : dProp Σ) }}}. *)
 
   (* Lemma wpc_incr (ℓa ℓb : loc) : *)
   (*   {{{ (True : dProp Σ) }}} *)
-  (*     incr ℓa ℓb @ 10; ⊤ *)
+  (*     incr_both ℓa ℓb @ 10; ⊤ *)
   (*   {{{ RET #(); (True : dProp Σ) }}} *)
   (*   {{{ (True : dProp Σ) }}}. *)
 
   Lemma incr_safe s k E ℓa ℓb :
-    ⊢ wpr s k E (incr ℓa ℓb) (recover ℓa ℓb) (λ _, True%I) (λ _ _, True%I).
+    ⊢ wpr s k E (incr_both ℓa ℓb) (recover ℓa ℓb) (λ _, True%I) (λ _ _, True%I).
   Proof.
   Abort.
 
